

HW2

Thursday, January 29, 2026 7:16 PM

1. $X_1 \dots X_n \sim \text{Gamma}(\alpha, \beta)$

a. $\frac{1}{\Gamma(\alpha)\beta^\alpha} x^{\alpha-1} e^{-x/\beta} = e^{\ln x^{\alpha-1} - \frac{1}{\beta} x} \frac{1}{\Gamma(\alpha)\beta^\alpha} = \frac{1}{\Gamma(\alpha)\beta^\alpha} e^{(\alpha-1)\ln(x) - \frac{1}{\beta} x}$
 $\eta_1 = \alpha \quad \alpha = \eta_1 \quad \eta_2 = -\frac{1}{\beta} \quad \beta = -\frac{1}{\eta_2} \Rightarrow \frac{\eta_1}{\Gamma(\eta_1)} e^{\eta_1 \ln(x) + \eta_2 x - \ln(x)}$

b. $\ell(\eta_1, \eta_2 | \underline{x}) = \sum_{i=1}^n \left[\eta_1 \ln(\eta_2) - \ln(\Gamma(\eta_1)) + \eta_1 \ln(x_i) - \eta_2 x_i - \ln(x_i) \right] = n \eta_1 \ln(\eta_2) - n \ln(\Gamma(\eta_1)) + \eta_1 \sum \ln(x_i) + \eta_2 \sum x_i - \sum \ln(x_i)$

$\frac{\partial}{\partial \eta_1} = n \ln(\eta_2) - n \frac{\Gamma'(\eta_1)}{\Gamma(\eta_1)} + \sum \ln(x_i) = 0 \Rightarrow \frac{1}{n} \sum \ln(x_i) = \frac{\Gamma'(\eta_1)}{\Gamma(\eta_1)} - \ln(\eta_2)$

$\frac{\partial}{\partial \eta_2} = \frac{n \eta_1}{-\eta_2} - \sum x_i = 0 \Rightarrow \frac{1}{n} \sum x_i = \frac{-\eta_1}{\eta_2}$

c. $\frac{1}{n} \sum \ln(x_i) = \frac{\Gamma'(\alpha)}{\Gamma(\alpha)} - \ln(\beta)$
 $\frac{1}{n} \sum x_i = \frac{\alpha}{\beta}$

2. $X_1, \dots, X_n \sim \text{Pois}(\lambda), \lambda > 0$

a. $\pi(\lambda) = \text{Gamma}(\alpha, \beta), \alpha, \beta > 0$

This is conjugate because the Poisson has the parameter λ something $\propto e^{\lambda(\text{parameter})}$, as does the Gamma, so they combine nicely into another thing that matches the Gamma Kernel

b. $f(y | \lambda) = \frac{\lambda^y e^{-\lambda}}{y!} \Rightarrow \pi(\lambda | y_i) = \prod_{i=1}^n \left[\frac{\lambda^{y_i} e^{-\lambda}}{y_i!} \right] \frac{\beta^\alpha}{\Gamma(\alpha)} \lambda^{\alpha-1} e^{-\beta \lambda}$
 $= \frac{\beta^\alpha}{\Gamma(\alpha) y_i!^n} \lambda^{\alpha + \sum y_i - 1} e^{-\lambda(1+\beta)}$

$= \frac{\beta^\alpha}{\Gamma(\alpha) y_i!^n} \frac{\Gamma(\alpha + \sum y_i)}{(1+\beta)^{\alpha + \sum y_i}} \text{Gamma}(\alpha + \sum y_i, 1+\beta)$

c. $M_{\text{EAN}}: \quad \bullet \quad (\alpha + \sum y_i) (1+\beta)^{-1}$

$\sqrt{\text{VAR}}: \quad \bullet \quad (\alpha + \sum y_i) (1+\beta)^{-2}$

3. $f(x|\theta) = \theta(1-\theta)^x \quad \theta \in (0,1) \quad x=0,1,2$

a. FIND MLE OF θ : $\ell(\theta, x) = \sum_{i=1}^n \ln(\theta) + x_i \ln(1-\theta) = n \ln(\theta) + \sum x_i \ln(1-\theta)$

$\frac{\partial}{\partial \theta} = \frac{n}{\theta} - \sum x_i \frac{1}{1-\theta} = 0 \Rightarrow \frac{n}{\theta} = \frac{\sum x_i}{1-\theta} \Rightarrow \frac{1}{\theta} = \frac{\sum x_i + n}{n}$

$$\begin{aligned} d\theta &= \frac{1}{1-\theta} = 0 \Rightarrow \eta - \eta\theta - \theta \sum x_i = 0 \quad \eta = \theta(n + \sum x_i) \quad \theta = \frac{\eta}{n + \sum x_i} = \frac{1}{\frac{n}{\eta} + \frac{1}{\sum x_i}} \\ &= \frac{1}{1 + \frac{1}{\eta} \sum x_i} \\ \frac{d^2}{d\theta^2} &\approx -\frac{\eta}{\theta^2} + \frac{\sum x_i}{(1-\theta)^2} \\ \hat{\theta} &= \frac{\eta}{n + \sum x_i} \end{aligned}$$

$$\begin{aligned} b. \quad \eta &= \frac{1-\theta}{\theta} \quad \theta\eta = 1-\theta \quad \theta(\eta+1) = 1 \quad \theta = \frac{1}{\eta+1} \\ \hat{\theta} &= \frac{\eta}{n + \sum x_i} \Rightarrow \frac{1}{\eta+1} = \frac{\eta}{n + \sum x_i} \quad \eta+1 = \frac{n + \sum x_i}{\eta} = 1 + \frac{\sum x_i}{\eta} \\ \Rightarrow \hat{\eta} &= \frac{\sum x_i}{\eta} \end{aligned}$$

$$c. \text{ Show ABOVE: } f(x|\eta) = \frac{1}{\eta+1} \left(1 - \frac{1}{\eta+1}\right)^x = \frac{1}{\eta+1} \left(\frac{\eta}{\eta+1}\right)^x = \frac{\eta^x}{(\eta+1)^{x+1}}$$

$$\begin{aligned} d. \quad \pi(\eta) &\propto \eta^{\alpha-1} (1+\eta)^{-\beta} \quad \eta > 0, 0 < \alpha < \beta \\ \pi(\eta|x) &\propto \prod_{i=1}^n \frac{\eta^{x_i}}{(\eta+1)^{x_i+1}} \eta^{\alpha-1} (1+\eta)^{-\beta} = \frac{\eta^{\sum x_i} \eta^{\alpha-1}}{(\eta+1)^{\sum x_i + n}} = \eta^{\alpha + \sum x_i - 1} (1+\eta)^{-(\beta + \sum x_i + n)} \\ &\text{SAME FORM AS PRIOR} \\ \int_0^\infty \eta^{\alpha + \sum x_i - 1} (1+\eta)^{-(\beta + \sum x_i + n)} d\eta &= 1 \end{aligned}$$

$$\text{BETA PRIOR: } a: \alpha + \sum x_i \quad \text{NEED } -a - b: \quad \alpha + \sum x_i + b = \beta + \sum x_i + n \\ b = \beta + \alpha + n$$

$$BP(\alpha + \sum x_i, \beta + \alpha + n)$$

$$c = \frac{\Gamma(\alpha + \sum x_i) \Gamma(\beta + \alpha + n)}{\Gamma(2\alpha + \beta + \sum x_i + n)}$$

$$e. \text{ WE JUST SHOWED THE POSTERIOR IS A } BP(\alpha + \sum x_i, \beta + \alpha + n)$$

$$\pi = E(\pi(\theta|x)) = \frac{\alpha + \sum x_i}{\beta + \alpha + n - 1}$$

$$\begin{aligned} f. \quad \int \frac{(t-\eta)^2}{\eta^2 (1+\eta)} \eta^{\alpha + \sum x_i - 1} (1+\eta)^{-(\beta + \sum x_i + n)} d\eta &= \int (t-\eta)^2 \eta^{\alpha + \sum x_i - 1} (1+\eta)^{-(\beta + \sum x_i + n + 2)} d\eta \\ a = \alpha + \sum x_i - 1 \quad -\beta - \sum x_i - n - 1 &= -a - \sum x_i + 1 - b \Rightarrow b = \beta + n - \alpha + 2 \end{aligned}$$

$$\pi = E(\pi(\theta|x)) = \frac{\alpha + \sum x_i - 1}{\beta + n - \alpha + 1}$$

In terms of parts e and f where we're supposed to plot the risk functions, I'm not really sure what we're supposed to be plotting. The parameter does not show up in the risk so I'm not sure what the variates are supposed to be...

$$4. \quad X_i | \theta \sim \text{Bern}(\theta) \quad \theta \in (0,1) \quad \pi(\theta) \sim \text{Unif}(0,1)$$

$$f(t) = \frac{(t-\theta)^2}{(1+\theta)^2} \quad (1 \leq t \leq 2)$$

$$\sim (0, \theta(1-\theta))$$

FIND BAYES RULE FOR ESTIMATION θ

$$\pi(\theta|x) \propto \text{BEW}(\theta) \text{ UNIF}(0,1) = \prod_{i=1}^n \theta^{x_i} (1-\theta)^{1-x_i} \cdot \frac{1}{1-0} = \theta^{\sum x_i} (1-\theta)^{n-\sum x_i}$$

$$r_{\pi} = \int \frac{(t-\theta)^2}{\theta(1-\theta)} \theta^{\sum x_i} (1-\theta)^{n-\sum x_i} d\theta = \int (t-\theta)^2 \underbrace{\theta^{\sum x_i - 1} (1-\theta)^{n-\sum x_i - 1}}_{\text{BETA}(\sum x_i, n-\sum x_i)} d\theta$$

$$\Rightarrow \pi(\theta|x) = \text{BETA}(\sum x_i, n-\sum x_i)$$

DUE TO LOSS OF $(t-\theta)^2$:

$$r_{\pi} = E(\pi(\theta|x)) = E(\text{BETA}) = \frac{\sum x_i}{\sum x_i + n - \sum x_i} = \frac{\sum x_i}{n} = \underline{\bar{x}}$$